backend/Deadcodeproof.v
@@ -507,7 +507,7 @@ Proof.
   instantiate (1 := nlive ge sp nm). auto.
   intros (tm' & P & Q).
   exists tm'; split. econstructor. econstructor; eauto.
-  eapply Mem.strong_non_private_stack_access_magree; eauto.
+  eapply Mem.public_stack_access_magree; eauto.
   eapply Mem.store_valid_access_3; eauto.
   auto.
 Qed.
@@ -805,7 +805,7 @@ Ltac UseTransfer :=
   constructor. eauto. constructor. eauto. constructor.
   eapply external_call_symbols_preserved. apply senv_preserved.
   simpl in B1; inv B1. simpl in B2; inv B2. econstructor; eauto.
-  eapply Mem.strong_non_private_stack_access_magree; eauto.
+  eapply Mem.public_stack_access_magree; eauto.
   erewrite <- list_forall2_length; eauto.
   eapply Mem.storebytes_range_perm; eauto.
   erewrite <- list_forall2_length; eauto.
