cfrontend/Cshmgenproof.v
@@ -988,11 +988,11 @@ Proof.
   apply alignof_blockcopy_1248.
   apply sizeof_pos.
   apply sizeof_alignof_blockcopy_compat.
-  (* PW: We need to prove that strong_non_private_stack_access m b for the memcpy extcall.
-   * Intuitively, this holds because we have non_private_stack_access (from storebytes);
+  (* PW: We need to prove that strong_stack_access m b for the memcpy extcall.
+   * Intuitively, this holds because we have stack_access (from storebytes);
    * AND the stack top does not have any frame information associated with it.
    *)
-  apply Mem.storebytes_non_private_stack_access in H9.
+  apply Mem.storebytes_stack_access in H9.
   destruct H9; auto.
   red. rewrite STACK_TOP_NO_INFO; auto. intuition.
   intuition.
